removing the typeclass for now

src/3d/prelude/Prelude.fsti
@@ -226,144 +226,103 @@ let max_int_sizes
     normalize_term_spec (max_int 10)
 
 
+
 (*
  * AR: scaffolding for getting arithmetic error locations in the 3d file
  *)
 
-open FStar.Mul
-
-noeq
-type t_uint = {
-  n   : nat;
-  t   : Type0;
-  v   : t -> FStar.UInt.uint_t n;
-  add : x:t -> y:t -> Pure t (requires UInt.size (v x + v y) n) (ensures fun z -> v z == v x + v y);
-  sub : x:t -> y:t -> Pure t (requires UInt.size (v x - v y) n) (ensures fun z -> v z == v x - v y);
-  mul : x:t -> y:t -> Pure t (requires UInt.size (v x * v y) n) (ensures fun z -> v z == v x * v y);
-  div : x:t -> y:t{v y =!= 0} -> Pure t (requires True)            (ensures fun z -> v z == v x / v y);
-}
-
-noextract
-let u_add (t:t_uint) (msg:string) (r:Prims.range) (x y:t.t)
-  : Pure t.t
-      (requires labeled r msg (UInt.size (t.v x + t.v y) t.n))
-      (ensures fun z -> t.v z == t.v x + t.v y)
-  = t.add x y
-
-noextract
-let u_sub (t:t_uint) (msg:string) (r:Prims.range) (x y:t.t)
-  : Pure t.t
-      (requires labeled r msg (UInt.size (t.v x - t.v y) t.n))
-      (ensures fun z -> t.v z == t.v x - t.v y)
-  = t.sub x y
-
-noextract
-let u_mul (t:t_uint) (msg:string) (r:Prims.range) (x y:t.t)
-  : Pure t.t
-      (requires labeled r msg (UInt.size (t.v x * t.v y) t.n))
-      (ensures fun z -> t.v z == t.v x * t.v y)
-  = t.mul x y
-
-noextract
-let u_div (t:t_uint) (msg:string) (r:Prims.range) (x y:t.t)
-  : Pure t.t
-      (requires labeled r msg (t.v y =!= 0))
-      (ensures fun z -> t.v z == t.v x / t.v y)
-  = t.div x y
-
-noextract
-let t_8 =
-  let open FStar.UInt8 in
-  { n = n; t = t; v = v; add = add; sub = sub; mul = mul; div = div }
-
-noextract
-let t_16 =
-  let open FStar.UInt16 in
-  { n = n; t = t; v = v; add = add; sub = sub; mul = mul; div = div }
-
-noextract
-let t_32 =
-  let open FStar.UInt32 in
-  { n = n; t = t; v = v; add = add; sub = sub; mul = mul; div = div }
-
-noextract
-let t_64 =
-  let open FStar.UInt64 in
-  { n = n; t = t; v = v; add = add; sub = sub; mul = mul; div = div }
-
-open FStar.Tactics
-
-noextract
-let norm () : Tac unit =
-  norm [iota; delta_only [
-    `%u_add; `%u_sub; `%u_mul; `%u_div;    
-    `%Mkt_uint?.n; `%Mkt_uint?.t; `%Mkt_uint?.v; `%Mkt_uint?.add; `%Mkt_uint?.sub; `%Mkt_uint?.mul; `%Mkt_uint?.div;
-    `%t_8; `%t_16; `%t_32; `%t_64 ]
-  ];
-  trefl ()
-
-unfold let msg_prefix : string = "Cannot verify the safety of "
-
-[@@postprocess_with norm]
 inline_for_extraction noextract
-let u8_add = u_add t_8 (String.concat "" [msg_prefix; "u8 addition"])
+val u8_add (r:Prims.range) (x y:UInt8.t)
+  : Pure UInt8.t
+      (requires labeled r "Cannot verify u8 addition" (UInt.size (UInt8.v x + UInt8.v y) UInt8.n))
+      (ensures fun z -> UInt8.v z == UInt8.v x + UInt8.v y)
 
-[@@postprocess_with norm]
 inline_for_extraction noextract
-let u16_add = u_add t_16 (String.concat "" [msg_prefix; "u16 addition"])
+val u8_sub (r:Prims.range) (x y:UInt8.t)
+  : Pure UInt8.t
+      (requires labeled r "Cannot verify u8 subtraction" (UInt.size (UInt8.v x - UInt8.v y) UInt8.n))
+      (ensures fun z -> UInt8.v z == UInt8.v x - UInt8.v y)
 
-[@@postprocess_with norm]
 inline_for_extraction noextract
-let u32_add = u_add t_32 (String.concat "" [msg_prefix; "u32 addition"])
+val u8_mul (r:Prims.range) (x y:UInt8.t)
+  : Pure UInt8.t
+      (requires labeled r "Cannot verify u8 multiplication" (UInt.size (UInt8.v x `Prims.op_Multiply` UInt8.v y) UInt8.n))
+      (ensures fun z -> UInt8.v z == UInt8.v x `Prims.op_Multiply` UInt8.v y)
 
-[@@postprocess_with norm]
 inline_for_extraction noextract
-let u64_add = u_add t_64 (String.concat "" [msg_prefix; "u64 addition"])
+val u8_div (r:Prims.range) (x y:UInt8.t)
+  : Pure UInt8.t
+      (requires labeled r "Cannot verify u8 division" (UInt8.v y =!= 0))
+      (ensures fun z -> UInt8.v z == UInt8.v x / UInt8.v y)
 
-[@@postprocess_with norm]
 inline_for_extraction noextract
-let u8_sub = u_sub t_8 (String.concat "" [msg_prefix; "u8 subtraction"])
+val u16_add (r:Prims.range) (x y:UInt16.t)
+  : Pure UInt16.t
+      (requires labeled r "Cannot verify u16 addition" (UInt.size (UInt16.v x + UInt16.v y) UInt16.n))
+      (ensures fun z -> UInt16.v z == UInt16.v x + UInt16.v y)
 
-[@@postprocess_with norm]
 inline_for_extraction noextract
-let u16_sub = u_sub t_16 (String.concat "" [msg_prefix; "u16 subtraction"])
+val u16_sub (r:Prims.range) (x y:UInt16.t)
+  : Pure UInt16.t
+      (requires labeled r "Cannot verify u16 subtraction" (UInt.size (UInt16.v x - UInt16.v y) UInt16.n))
+      (ensures fun z -> UInt16.v z == UInt16.v x - UInt16.v y)
 
-[@@postprocess_with norm]
 inline_for_extraction noextract
-let u32_sub = u_sub t_32 (String.concat "" [msg_prefix; "u32 subtraction"])
+val u16_mul (r:Prims.range) (x y:UInt16.t)
+  : Pure UInt16.t
+      (requires labeled r "Cannot verify u16 multiplication" (UInt.size (UInt16.v x `Prims.op_Multiply` UInt16.v y) UInt16.n))
+      (ensures fun z -> UInt16.v z == UInt16.v x `Prims.op_Multiply` UInt16.v y)
 
-[@@postprocess_with norm]
 inline_for_extraction noextract
-let u64_sub = u_sub t_64 (String.concat "" [msg_prefix; "u64 subtraction"])
+val u16_div (r:Prims.range) (x y:UInt16.t)
+  : Pure UInt16.t
+      (requires labeled r "Cannot verify u16 division" (UInt16.v y =!= 0))
+      (ensures fun z -> UInt16.v z == UInt16.v x / UInt16.v y)
 
-[@@postprocess_with norm]
 inline_for_extraction noextract
-let u8_mul = u_mul t_8 (String.concat "" [msg_prefix; "u8 multiplication"])
+val u32_add (r:Prims.range) (x y:UInt32.t)
+  : Pure UInt32.t
+      (requires labeled r "Cannot verify u32 addition" (UInt.size (UInt32.v x + UInt32.v y) UInt32.n))
+      (ensures fun z -> UInt32.v z == UInt32.v x + UInt32.v y)
 
-[@@postprocess_with norm]
 inline_for_extraction noextract
-let u16_mul = u_mul t_16 (String.concat "" [msg_prefix; "u16 multiplication"])
+val u32_sub (r:Prims.range) (x y:UInt32.t)
+  : Pure UInt32.t
+      (requires labeled r "Cannot verify u32 subtraction" (UInt.size (UInt32.v x - UInt32.v y) UInt32.n))
+      (ensures fun z -> UInt32.v z == UInt32.v x - UInt32.v y)
 
-[@@postprocess_with norm]
 inline_for_extraction noextract
-let u32_mul = u_mul t_32 (String.concat "" [msg_prefix; "u32 multiplication"])
+val u32_mul (r:Prims.range) (x y:UInt32.t)
+  : Pure UInt32.t
+      (requires labeled r "Cannot verify u32 multiplication" (UInt.size (UInt32.v x `Prims.op_Multiply` UInt32.v y) UInt32.n))
+      (ensures fun z -> UInt32.v z == UInt32.v x `Prims.op_Multiply` UInt32.v y)
 
-[@@postprocess_with norm]
 inline_for_extraction noextract
-let u64_mul = u_mul t_64 (String.concat "" [msg_prefix; "u64 multiplication"])
+val u32_div (r:Prims.range) (x y:UInt32.t)
+  : Pure UInt32.t
+      (requires labeled r "Cannot verify u32 division" (UInt32.v y =!= 0))
+      (ensures fun z -> UInt32.v z == UInt32.v x / UInt32.v y)
 
-[@@postprocess_with norm]
 inline_for_extraction noextract
-let u8_div = u_div t_8 (String.concat "" [msg_prefix; "u8 division"])
+val u64_add (r:Prims.range) (x y:UInt64.t)
+  : Pure UInt64.t
+      (requires labeled r "Cannot verify u64 addition" (UInt.size (UInt64.v x + UInt64.v y) UInt64.n))
+      (ensures fun z -> UInt64.v z == UInt64.v x + UInt64.v y)
 
-[@@postprocess_with norm]
 inline_for_extraction noextract
-let u16_div = u_div t_16 (String.concat "" [msg_prefix; "u16 division"])
+val u64_sub (r:Prims.range) (x y:UInt64.t)
+  : Pure UInt64.t
+      (requires labeled r "Cannot verify u64 subtraction" (UInt.size (UInt64.v x - UInt64.v y) UInt64.n))
+      (ensures fun z -> UInt64.v z == UInt64.v x - UInt64.v y)
 
-[@@postprocess_with norm]
 inline_for_extraction noextract
-let u32_div = u_div t_32 (String.concat "" [msg_prefix; "u32 division"])
+val u64_mul (r:Prims.range) (x y:UInt64.t)
+  : Pure UInt64.t
+      (requires labeled r "Cannot verify u64 multiplication" (UInt.size (UInt64.v x `Prims.op_Multiply` UInt64.v y) UInt64.n))
+      (ensures fun z -> UInt64.v z == UInt64.v x `Prims.op_Multiply` UInt64.v y)
 
-[@@postprocess_with norm]
 inline_for_extraction noextract
-let u64_div = u_div t_64 (String.concat "" [msg_prefix; "u64 division"])
+val u64_div (r:Prims.range) (x y:UInt64.t)
+  : Pure UInt64.t
+      (requires labeled r "Cannot verify u64 division" (UInt64.v y =!= 0))
+      (ensures fun z -> UInt64.v z == UInt64.v x / UInt64.v y)
